Sync AST with plutus compiler as of 2023-12-01 * Include new builtin functions and constant types * Adjust representation of SomeTypeIn for constant types * Add Data for builtin data * Replace handwritten eqb and eqb_eq proofs

src/PlutusIR/Analysis/Equality.v
@@ -11,18 +11,39 @@ From PlutusCert Require Import
   Util.List
 .
 
-Set Implicit Arguments.
-
 Definition EqDec := fun A : Type => forall x y : A, {x = y} + {x <> y}.
 
+Definition Z_eq_dec := Z.eq_dec.
 
 Create HintDb Eqs.
-#[export] Hint Resolve Nat.eq_dec Z.eq_dec ascii_dec bool_dec string_dec list_eq_dec : Eqs.
+#[export] Hint Resolve
+  Nat.eq_dec Z.eq_dec ascii_dec bool_dec string_dec list_eq_dec
+  Pos.eq_dec
+  : Eqs
+.
+
 
 Ltac solveEq :=
   intros;
   unfold EqDec;
-  decide equality; auto with Eqs. (* debug auto with Eqs.*)
+  decide equality;
+  auto with Eqs (* debug auto with Eqs.*)
+.
+
+
+(* work-around to let auto convert between
+  EqDec A and its definition forall x y : A, {x = y} + {x <> y} := id.
+*)
+Definition conv A : EqDec A -> forall x y : A, {x = y} + {x <> y} := id.
+Definition conv' A : (forall x y : A, {x = y} + {x <> y}) -> EqDec A := id.
+  #[export] Hint Resolve 10 conv conv' : Eqs.
+
+
+Definition prod_dec A B : EqDec A -> EqDec B -> EqDec (A * B).
+solveEq.
+Defined.
+  #[export] Hint Resolve prod_dec : Eqs.
+
 
 Definition unit_dec: EqDec unit. Proof. solveEq. Defined.
   #[export] Hint Resolve unit_dec : Eqs.
@@ -39,10 +60,32 @@ Definition func_dec : EqDec DefaultFun. Proof. solveEq. Defined.
 Definition DefaultUni_dec : EqDec DefaultUni. solveEq. Defined.
   #[export] Hint Resolve DefaultUni_dec : Eqs.
 
-Definition uniType_dec : forall t, EqDec (uniType t). intro t. destruct t; simpl; solveEq; solveEq. Defined.
-  #[export] Hint Resolve uniType_dec : Eqs.
 
-Definition valueOf_dec : forall t, EqDec (valueOf t). solveEq. apply uniType_dec. Defined.
+Fixpoint Data_dec (x y : Data) : {x = y} + {x <> y}.
+  unfold EqDec.
+  decide equality.
+  all: auto with Eqs.
+Defined.
+  #[export] Hint Resolve Data_dec : Eqs.
+
+Definition uniType_dec : forall (t : DefaultUni), EqDec (uniType t).
+  unfold uniType.
+  intro t.
+  apply uniType_option_rect.
+  all: intros; try solveEq.
+  - rewrite e1 in *. clear e1.
+    intuition.
+  - rewrite e2 in *.
+    rewrite e3 in *.
+    intuition.
+  - rewrite e2 in *.
+    rewrite e3 in *.
+    intuition.
+Defined.
+#[export] Hint Resolve uniType_dec : Eqs.
+
+Definition valueOf_dec : forall t, EqDec (valueOf t). solveEq.
+Defined.
   #[export] Hint Resolve valueOf_dec : Eqs.
 
 Definition typeIn_dec : forall t, EqDec (typeIn t). solveEq. Defined.
@@ -110,6 +153,77 @@ Definition pass_dec (name_dec : EqDec name) (p1 p2 : pass) :
 
 Definition pair_dec {a b} (a_dec : EqDec a) (b_dec : EqDec b) : EqDec (a * b).
   Proof. solveEq. Defined.
+
+
+
+Section Derived_Eqb.
+  (*
+    I got tired of the handwritten boolean equality that have to be
+    updated with every change in AST (including soundness proofs). They are implied
+    by the above definitions.
+
+    If it turns out that these are significantly worse in terms of performance, reconsider
+    this approach.
+  *)
+
+
+  Definition Eqb x := x -> x -> bool.
+  Definition eq_dec_to_eqb {A} : EqDec A -> Eqb A :=
+    fun dec_eq x y =>  match dec_eq x y with
+    | left _ => true
+    | right _ => false
+    end.
+
+  Definition func_eqb : Eqb DefaultFun := eq_dec_to_eqb func_dec.
+  Definition unit_eqb : Eqb unit := eq_dec_to_eqb unit_dec.
+  Definition strictness_eqb : Eqb strictness := eq_dec_to_eqb strictness_dec.
+  Definition recursivity_eqb : Eqb recursivity := eq_dec_to_eqb recursivity_dec.
+  Definition DefaultUni_eqb : Eqb DefaultUni := eq_dec_to_eqb DefaultUni_dec.
+  Definition uniType_eqb : forall t, Eqb (uniType t) := fun t => eq_dec_to_eqb (uniType_dec t).
+  Definition valueOf_eqb : forall t, Eqb (valueOf t) := fun t => eq_dec_to_eqb (valueOf_dec t).
+  Definition some_valueOf_eqb: Eqb (@some valueOf) := eq_dec_to_eqb (some_valueOf_dec).
+  Definition typeIn_eqb : forall t, Eqb (typeIn t) := fun t => eq_dec_to_eqb (typeIn_dec t).
+  Definition some_typeIn_eqb : Eqb (@some typeIn) := eq_dec_to_eqb (some_typeIn_dec).
+  Definition Kind_eqb : Eqb kind := eq_dec_to_eqb Kind_dec.
+  Definition Ty_eqb : Eqb ty := eq_dec_to_eqb Ty_dec.
+  Definition TVDecl_eqb : Eqb tvdecl := eq_dec_to_eqb TVDecl_dec.
+  Definition VDecl_eqb: Eqb vdecl := eq_dec_to_eqb VDecl_dec.
+  Definition DTDecl_eqb: Eqb dtdecl := eq_dec_to_eqb DTDecl_dec.
+  Definition Term_eqb : Eqb term := eq_dec_to_eqb term_dec.
+  Definition Binding_eqb : Eqb binding := eq_dec_to_eqb binding_dec.
+
+  Definition eq_dec_to_eqb__sound {A} (dec : EqDec A)
+    : forall (x y : A), (eq_dec_to_eqb dec) x y = true <-> x = y.
+  Proof.
+    unfold eq_dec_to_eqb.
+    intros x y.
+    destruct (dec x y).
+    - subst. intuition.
+    - intuition.
+      inversion H.
+  Qed.
+
+  Definition func_eqb_eq := eq_dec_to_eqb__sound func_dec.
+  Definition unit_eqb_eq := eq_dec_to_eqb__sound unit_dec.
+  Definition strictness_eqb_eq := eq_dec_to_eqb__sound strictness_dec.
+  Definition recursivity_eqb_eq := eq_dec_to_eqb__sound recursivity_dec.
+  Definition DefaultUni_eqb_eq := eq_dec_to_eqb__sound DefaultUni_dec.
+  Definition uniType_eqb_eq := fun t => eq_dec_to_eqb__sound (uniType_dec t).
+  Definition valueOf_eqb_eq := fun t => eq_dec_to_eqb__sound (valueOf_dec t).
+  Definition some_valueOf_eqb_eq := eq_dec_to_eqb__sound (some_valueOf_dec).
+  Definition typeIn_eqb_eq := fun t => eq_dec_to_eqb__sound (typeIn_dec t).
+  Definition some_typeIn_eqb_eq := eq_dec_to_eqb__sound (some_typeIn_dec).
+  Definition Kind_eqb_eq := eq_dec_to_eqb__sound Kind_dec.
+  Definition Ty_eqb_eq := eq_dec_to_eqb__sound Ty_dec.
+  Definition TVDecl_eqb_eq := eq_dec_to_eqb__sound TVDecl_dec.
+  Definition VDecl_eqb_eq := eq_dec_to_eqb__sound VDecl_dec.
+  Definition DTDecl_eqb_eq := eq_dec_to_eqb__sound DTDecl_dec.
+  Definition Term_eqb_eq := eq_dec_to_eqb__sound term_dec.
+  Definition Binding_eqb_eq := eq_dec_to_eqb__sound binding_dec.
+
+
+End Derived_Eqb.
+
 (* boolean equality
 I define this separately from the dec_* functions to avoid carrying around
 proof terms at run-time.
@@ -122,6 +236,47 @@ proof terms at run-time.
 
 Create HintDb reflection.
 
+#[export] Hint Resolve ->
+  func_eqb_eq
+  unit_eqb_eq
+  strictness_eqb_eq
+  recursivity_eqb_eq
+  DefaultUni_eqb_eq
+  uniType_eqb_eq
+  valueOf_eqb_eq
+  some_valueOf_eqb_eq
+  typeIn_eqb_eq
+  some_typeIn_eqb_eq
+  Kind_eqb_eq
+  Ty_eqb_eq
+  TVDecl_eqb_eq
+  VDecl_eqb_eq
+  DTDecl_eqb_eq
+  Term_eqb_eq
+  Binding_eqb_eq
+  : reflection
+.
+
+#[export] Hint Resolve <-
+  func_eqb_eq
+  unit_eqb_eq
+  strictness_eqb_eq
+  recursivity_eqb_eq
+  DefaultUni_eqb_eq
+  uniType_eqb_eq
+  valueOf_eqb_eq
+  some_valueOf_eqb_eq
+  typeIn_eqb_eq
+  some_typeIn_eqb_eq
+  Kind_eqb_eq
+  Ty_eqb_eq
+  TVDecl_eqb_eq
+  VDecl_eqb_eq
+  DTDecl_eqb_eq
+  Term_eqb_eq
+  Binding_eqb_eq
+  : reflection
+.
 (*
   Note [#[export] Hints and name-collision]
   ~~~~~~~~~~~~~~~~
@@ -155,412 +310,3 @@ Definition string_eqb_eq := String.eqb_eq.
 : reflection.
 Definition andb_and : forall s t, s && t = true -> s = true /\ t = true.
 Proof. auto with reflection. Qed.
-
-Ltac rewrite_eqbs := repeat (
-  match goal with
-  | Hyp : _ |- _ => apply andb_and in Hyp
-  end).
-
-(* Destruct all /\ hypotheses*)
-Ltac destruct_ands := repeat (
-  match goal with
-  | Hyp : ?l /\ ?r |- _ => destruct Hyp
-  end).
-
-Ltac bool_assumptions :=
-  repeat (rewrite_eqbs; destruct_ands).
-
-Ltac eqb_eq_tac :=
-  intros x y;
-  constructor; (* <-> *)
-
-  (* -> case*)
-  [ generalize y; clear y; induction x; intros y; (* get suitable IH *)
-    destruct y;
-    intros H;
-    repeat (rewrite_eqbs; destruct_ands); (* unfolds the call and rewrites && into /\*)
-    (f_equal || inversion H); (* Eliminate cases based on H, f_equal on same constructors*)
-    eauto with reflection
-
-  (* <- case *)
-  | intros H;
-    subst x;
-    induction y;
-    simpl;
-    eauto with reflection
-  ].
-
-
-Definition Eqb x := x -> x -> bool.
-(*
-Definition Eqb_eq := fun {a} (eqb : Eqb a) => forall (x y : a),
-  eqb x y = true <-> x = y.
-  *)
-
-Definition unit_eqb: Eqb unit := fun x y => match x, y with
-  | tt, tt => true
-  end.
-Definition unit_eqb_eq : forall u u', unit_eqb u u' = true <-> u = u'.
-   Proof. eqb_eq_tac. Defined.
-
-#[export] Hint Resolve -> unit_eqb_eq : reflection.
-#[export] Hint Resolve <- unit_eqb_eq : reflection.
-
-
-Definition strictness_eqb: Eqb strictness := fun x y =>
-  match x, y with
-  | NonStrict, NonStrict => true
-  | Strict   , Strict    => true
-  | _, _                 => false
-  end.
-
-Definition strictness_eqb_eq : forall s s', strictness_eqb s s' = true <-> s = s'.
-Proof. eqb_eq_tac. Defined.
-#[export] Hint Resolve -> strictness_eqb_eq : reflection.
-#[export] Hint Resolve <- strictness_eqb_eq : reflection.
-
-Definition recursivity_eqb : Eqb recursivity := fun x y => match x, y with
-  | NonRec, NonRec => true
-  | Rec, Rec => true
-  | _, _ => false
-  end.
-
-Definition recursivity_eqb_eq : forall r r', recursivity_eqb r r' = true <-> r = r'.
-Proof. eqb_eq_tac. Qed.
-#[export] Hint Resolve -> recursivity_eqb_eq : reflection.
-#[export] Hint Resolve <- recursivity_eqb_eq : reflection.
-
-Definition func_eqb : Eqb DefaultFun := fun x y => match x, y with
-  | AddInteger , AddInteger => true
-  | SubtractInteger , SubtractInteger => true
-  | MultiplyInteger , MultiplyInteger => true
-  | DivideInteger , DivideInteger => true
-  | QuotientInteger , QuotientInteger => true
-  | RemainderInteger , RemainderInteger => true
-  | ModInteger , ModInteger => true
-  | LessThanInteger , LessThanInteger => true
-  | LessThanEqInteger , LessThanEqInteger => true
-  | GreaterThanInteger , GreaterThanInteger => true
-  | GreaterThanEqInteger , GreaterThanEqInteger => true
-  | EqInteger , EqInteger => true
-  | Concatenate , Concatenate => true
-  | TakeByteString , TakeByteString => true
-  | DropByteString , DropByteString => true
-  | SHA2 , SHA2 => true
-  | SHA3 , SHA3 => true
-  | VerifySignature , VerifySignature => true
-  | EqByteString , EqByteString => true
-  | LtByteString , LtByteString => true
-  | GtByteString , GtByteString => true
-  | IfThenElse , IfThenElse => true
-  | CharToString , CharToString => true
-  | Append , Append => true
-  | Trace , Trace => true
-  | _, _ => false
-  end.
-
-Definition func_eqb_eq : forall f f', func_eqb f f' = true <-> f = f'.
-Proof. eqb_eq_tac. Qed.
-#[export] Hint Resolve -> func_eqb_eq : reflection.
-#[export] Hint Resolve <- func_eqb_eq : reflection.
-
-Definition DefaultUni_eqb : Eqb DefaultUni := fun x y => match x, y with
-  | DefaultUniInteger , DefaultUniInteger => true
-  | DefaultUniByteString , DefaultUniByteString => true
-  | DefaultUniString , DefaultUniString => true
-  | DefaultUniChar , DefaultUniChar => true
-  | DefaultUniUnit , DefaultUniUnit => true
-  | DefaultUniBool , DefaultUniBool => true
-  | _, _ => false
-  end.
-
-Definition DefaultUni_eqb_eq : forall u u', DefaultUni_eqb u u' = true <-> u = u'.
-Proof. eqb_eq_tac. Qed.
-#[export] Hint Resolve -> DefaultUni_eqb_eq : reflection.
-#[export] Hint Resolve <- DefaultUni_eqb_eq : reflection.
-
-Definition uniType_eqb : forall t, Eqb (uniType t) := fun ty =>
-  match ty return Eqb (uniType ty) with
-  | DefaultUniInteger => Z.eqb
-  | DefaultUniChar    => Strings.Ascii.eqb
-  | DefaultUniUnit    => unit_eqb
-  | DefaultUniBool    => Bool.eqb
-  | DefaultUniByteString => String.eqb
-  | DefaultUniString    => String.eqb
-  end.
-
-Definition uniType_eqb_eq : forall t ty ty', uniType_eqb t ty ty' = true <-> ty = ty'.
-Proof.
-  intro t.
-  destruct t;
-  auto using Z.eqb_eq, string_eqb_eq, unit_eqb_eq, Ascii.eqb_eq, Nat.eqb_eq, Bool.eqb_true_iff.
-Qed.
-
-#[export] Hint Resolve -> uniType_eqb_eq : reflection.
-#[export] Hint Resolve <- uniType_eqb_eq : reflection.
-
-Definition valueOf_eqb : forall t, Eqb (valueOf t) := fun ty x y => match x, y with
-  | ValueOf _ x, ValueOf _ y => uniType_eqb ty x y
-  end.
-
-Definition valueOf_eqb_eq : forall t c c', @valueOf_eqb t c c' = true <-> c = c'.
-Proof.
-  intros t.
-  destruct t;
-  eqb_eq_tac.
-Qed.
-#[export] Hint Resolve -> valueOf_eqb_eq : reflection.
-#[export] Hint Resolve <- valueOf_eqb_eq : reflection.
-
-Definition some_valueOf_eqb: Eqb (@some valueOf) := fun x y => match x, y with
-  | @Some' _ t v, @Some' _ t' v' =>
-    match DefaultUni_dec t t' with
-    | left H => valueOf_eqb (eq_rect _ valueOf v _ H) v'
-    | _      => false
-    end
-  end.
-
-Definition some_valueOf_eqb_eq : forall v v', some_valueOf_eqb v v' = true <-> v = v'.
-Proof.
-  eqb_eq_tac.
-  - destruct u, u0;
-    simpl in *;
-    f_equal;
-    inversion H;
-    auto with reflection.
-  - destruct u;
-    simpl;
-    destruct f; simpl;
-    auto with reflection.
-Qed.
-#[export] Hint Resolve -> some_valueOf_eqb_eq : reflection.
-#[export] Hint Resolve <- some_valueOf_eqb_eq : reflection.
-
-Definition typeIn_eqb : forall t, Eqb (typeIn t) := fun ty x y => match x, y with
-  | @TypeIn _, TypeIn _ => true
-  end.
-
-Definition typeIn_eqb_eq : forall t ty ty', @typeIn_eqb t ty ty' = true <-> ty = ty'.
-Proof.
-  intros t.
-  destruct t;
-  eqb_eq_tac.
-Qed.
-#[export] Hint Resolve -> typeIn_eqb_eq : reflection.
-#[export] Hint Resolve <- typeIn_eqb_eq : reflection.
-
-Definition some_typeIn_eqb : Eqb (@some typeIn) := fun x y => match x, y with
-  | @Some' _ t v, @Some' _ t' v' =>
-    match DefaultUni_dec t t' with
-    | left H => typeIn_eqb (eq_rect _ typeIn v _ H) v'
-    | _      => false
-    end
-  end.
-
-Definition some_typeIn_eqb_eq : forall ty ty', some_typeIn_eqb ty ty' = true <-> ty = ty'.
-Proof.
-  eqb_eq_tac.
-  - destruct u, u0;
-    simpl in *;
-    f_equal;
-    inversion H;
-    auto with reflection.
-  - destruct u;
-    simpl;
-    destruct f; simpl;
-    auto with reflection.
-Qed.
-#[export] Hint Resolve -> some_typeIn_eqb_eq : reflection.
-#[export] Hint Resolve <- some_typeIn_eqb_eq : reflection.
-
-Fixpoint Kind_eqb (x y : kind) : bool := match x, y with
-  | Kind_Base, Kind_Base => true
-  | Kind_Arrow K1 K2, Kind_Arrow K3 K4 => Kind_eqb K1 K3 && Kind_eqb K2 K4
-  | _, _ => false
-  end.
-
-Definition Kind_eqb_eq : forall k k', Kind_eqb k k' = true <-> k = k'.
-Proof. eqb_eq_tac. Defined.
-
-#[export] Hint Resolve -> Kind_eqb_eq : reflection.
-#[export] Hint Resolve <- Kind_eqb_eq : reflection.
-
-(* TODO: This is not correct yet. Because we have computation in types, we can not merely rely
-  on syntactic equality checking. *)
-Fixpoint Ty_eqb (x y : ty) : bool := match x, y with
-  | Ty_Var X, Ty_Var Y => String.eqb X Y
-  | Ty_Fun T1 T2, Ty_Fun T3 T4 => Ty_eqb T1 T3 && Ty_eqb T2 T4
-  | Ty_IFix T1 U1, Ty_IFix T2 U2 => Ty_eqb T1 T2 && Ty_eqb U1 U2
-  | Ty_Forall X1 K1 T1, Ty_Forall X2 K2 T2 => String.eqb X1 X2 && Kind_eqb K1 K2 && Ty_eqb T1 T2
-  | Ty_Builtin s1, Ty_Builtin s2 => some_typeIn_eqb s1 s2
-  | Ty_Lam X1 K1 T1, Ty_Lam X2 K2 T2 => String.eqb X1 X2 && Kind_eqb K1 K2 && Ty_eqb T1 T2
-  | Ty_App S1 T1, Ty_App S2 T2 => Ty_eqb S1 S2 && Ty_eqb T1 T2
-  | _, _ => false
-  end.
-
-Definition Ty_eqb_eq : forall ty ty', Ty_eqb ty ty' = true <-> ty = ty'.
-Proof. Local Open Scope string_scope. eqb_eq_tac; try (inversion H).
-  - assert (b =? b = true) by eauto with reflection.
-    assert (Kind_eqb k k = true) by eauto with reflection.
-    rewrite H. rewrite H0. rewrite IHy. auto.
-  - assert (b =? b = true) by eauto with reflection.
-    assert (Kind_eqb k k = true) by eauto with reflection.
-    rewrite H. rewrite H0. rewrite IHy. auto.
-Defined.
-#[export] Hint Resolve -> Ty_eqb_eq : reflection.
-#[export] Hint Resolve <- Ty_eqb_eq : reflection.
-
-
-Definition TVDecl_eqb : Eqb tvdecl := fun x y => match x, y with
-  | TyVarDecl ty k, TyVarDecl ty' k' => String.eqb ty ty' && Kind_eqb k k'
-  end.
-
-Definition TVDecl_eqb_eq : forall tvd tvd', TVDecl_eqb tvd tvd' = true <-> tvd = tvd'.
-Proof. eqb_eq_tac. Defined.
-#[export] Hint Resolve -> TVDecl_eqb_eq : reflection.
-#[export] Hint Resolve <- TVDecl_eqb_eq : reflection.
-
-
-Definition VDecl_eqb: Eqb vdecl := fun x y => match x, y with
-  | VarDecl x ty, VarDecl x' ty' => String.eqb x x' && Ty_eqb ty ty'
-  end.
-Definition VDecl_eqb_eq : forall vd vd', VDecl_eqb vd vd' = true <-> vd = vd'.
-Proof. eqb_eq_tac. Defined.
-
-#[export] Hint Resolve -> VDecl_eqb_eq : reflection.
-#[export] Hint Resolve <- VDecl_eqb_eq : reflection.
-(* reminder: String.eqb_eq is opaque, perhaps this will be an
-issue later on*)
-
-Definition list_eqb a (eqb : Eqb a) : Eqb (list a) := fix f xs ys :=
-  match xs, ys with
-  | nil, nil             => true
-  | cons x xs, cons y ys => eqb x y && f xs ys
-  | _, _                 => false
-  end.
-
-Lemma list_eqb_tl A eqb (x y : A) (xs ys : list A) : list_eqb eqb (x :: xs) (y :: ys) = true -> list_eqb eqb xs ys = true.
-Proof.
-  simpl. intros. rewrite andb_true_iff in H. intuition.
-Qed.
-
-
-(* Instead of requiring a general decidable equality eqb x x' <-> x = x', we require
-   that the elements in the list xs have decidable equality. This makes mutual
-   inductive proofs possible *)
-Definition list_eqb_eq_Forall a (a_eqb : Eqb a) xs xs' (H_sound_xs : Forall (fun x => forall x', a_eqb x x' = true <-> x = x') xs) :
-  list_eqb a_eqb xs xs' = true <-> xs = xs'.
-Proof.
-  revert xs'.
-  induction xs.
-  intros xs'.
-  - simpl.
-    destruct xs'; split; inversion 1; reflexivity.
-  - simpl.
-    destruct xs'; split; try solve [inversion 1].
-    + intros H_eqb.
-      rewrite andb_true_iff in H_eqb. destruct H_eqb.
-      inversion_clear H_sound_xs.
-      specialize (IHxs H2).
-      rewrite H1 in H. subst.
-      specialize (IHxs xs').
-      destruct IHxs.
-      f_equal.
-      auto.
-    + intros.
-      inversion H; subst.
-      rewrite andb_true_iff.
-      inversion H_sound_xs; subst.
-      rewrite H2.
-      rewrite IHxs; auto.
-Qed.
-
-Arguments list_eqb_eq_Forall {a} _ _ _ _.
-
-(* This is the more specific version that isn't suitable for mutual induction *)
-Definition list_eqb_eq A (A_eqb : Eqb A) (H : forall x x', A_eqb x x' = true <-> x = x') : forall xs xs',
-  list_eqb A_eqb xs xs' = true <-> xs = xs'.
-Proof.
-  intros.
-  assert (H_sound_xs : Forall (fun x => forall x', A_eqb x x' = true <-> x = x') xs).
-  { induction xs.
-    + constructor.
-    + constructor.
-      * specialize (H a).
-        assumption.
-      * assumption.
-  }
-  apply list_eqb_eq_Forall. auto.
-Qed.
-
-
-#[export] Hint Resolve -> list_eqb_eq : reflection.
-#[export] Hint Resolve <- list_eqb_eq : reflection.
-
-Definition DTDecl_eqb: Eqb dtdecl := fun x y => match x, y with
-  | Datatype tvd tvds n cs, Datatype tvd' tvds' n' cs' =>
-    TVDecl_eqb tvd tvd' && list_eqb TVDecl_eqb tvds tvds'
-      && String.eqb n n' && list_eqb VDecl_eqb cs cs'
-    end.
-Definition DTDecl_eqb_eq : forall dtd dtd', DTDecl_eqb dtd dtd' = true <-> dtd = dtd'.
-Proof.
-  eqb_eq_tac.
-  - apply (list_eqb_eq _ TVDecl_eqb_eq ).
-    assumption.
-  - apply (list_eqb_eq _ VDecl_eqb_eq).
-    assumption.
-  - repeat (apply andb_true_iff_proj_r2l; constructor);
-     auto with reflection.
-    + apply (list_eqb_eq _ TVDecl_eqb_eq).
-      reflexivity.
-    + apply (list_eqb_eq _ VDecl_eqb_eq).
-      reflexivity.
-Qed.
-#[export] Hint Resolve -> DTDecl_eqb_eq : reflection.
-#[export] Hint Resolve <- DTDecl_eqb_eq : reflection.
-
-
-
-
-
-
-
-Fixpoint Term_eqb (x y : term) {struct x} : bool := match x, y with
-  | Let rec bs t, Let rec' bs' t' => recursivity_eqb rec rec'
-      && list_eqb Binding_eqb bs bs'
-        && Term_eqb t t'
-  | Let _ _ _, _ => false
-  | Var n, Var n' => String.eqb n n'
-  | Var _, _ => false
-  | TyAbs n k t, TyAbs n' k' t' => String.eqb n n' && Kind_eqb k k' && Term_eqb t t'
-  | TyAbs _ _ _, _ => false
-  | LamAbs n ty t, LamAbs n' ty' t' => String.eqb n n' && Ty_eqb ty ty' && Term_eqb t t'
-  | LamAbs _ _ _, _ => false
-  | Apply s t, Apply s' t' => Term_eqb s s' && Term_eqb t t'
-  | Apply _ _, _ => false
-  | Constant c, Constant c' => some_valueOf_eqb c c'
-  | Constant _, _ => false
-  | Builtin f, Builtin f' => func_eqb f f'
-  | Builtin _, _ => false
-  | TyInst t ty, TyInst t' ty' => Term_eqb t t' && Ty_eqb ty ty'
-  | TyInst _ _, _ => false
-  | Error ty , Error ty' => Ty_eqb ty ty'
-  | Error _, _ => false
-  | IWrap ty1 ty2 t, IWrap ty1' ty2' t' => Ty_eqb ty1 ty1' && Ty_eqb ty2 ty2' && Term_eqb t t'
-  | IWrap _ _ _, _ => false
-  | Unwrap t, Unwrap t' => Term_eqb t t'
-  | Unwrap _, _ => false
-  | Constr n args, Constr n' args' => Nat.eqb n n' && forall2b Term_eqb args args'
-  | Constr _ _ , _ => false
-  | Case t ts, Case t' ts' => Term_eqb t t' && forall2b Term_eqb ts ts'
-  | Case _ _, _ => false
-  end
-with Binding_eqb (x y : binding) {struct x} : bool := match x, y with
-  | TermBind s vd t, TermBind s' vd' t' => strictness_eqb s s' && VDecl_eqb vd vd' && Term_eqb t t'
-  | TermBind _ _ _, _ => false
-  | TypeBind tvd ty, TypeBind tvd' ty' => TVDecl_eqb tvd tvd' && Ty_eqb ty ty'
-  | TypeBind _ _, _ => false
-  | DatatypeBind  dtd, DatatypeBind dtd' => DTDecl_eqb dtd dtd'
-  | DatatypeBind _, _ => false
-  end
-  .
