src/PlutusIR/Semantics/Dynamic/Bigstep/EvalToValue.v
@@ -10,6 +10,9 @@ Lemma compute_defaultfun__to_value : forall t v,
 Proof with (try discriminate).
   intros.
   destruct t...
+  (* TODO: redo for new built-ins *)
+  admit.
+  (*
   simpl in H0.
   all: destruct t1...
   all: try destruct t1_1...
@@ -48,7 +51,8 @@ Proof with (try discriminate).
   all: try (inversion H0; subst)...
   all: autounfold.
   all: try constructor.
-Qed.
+  *)
+Admitted.
 
 Lemma eval_to_value :
     (forall t v k, t =[k]=> v -> value v) /\
@@ -67,8 +71,8 @@ Proof with (eauto with hintdb__eval_no_error).
     all: constructor...
     all: constructor...
     all: try solve [intros Hcon; inversion Hcon].
-    all: unfold arity...
-Qed.
+    admit. (* TODO: implement arity *)
+Admitted.
 
 Corollary eval_to_value__eval : forall t v k,
     t =[k]=> v ->
